compiler/wasm/wbf_thmsScript.sml
@@ -10,20 +10,24 @@ val ssa  =          [GSYM APPEND_ASSOC, Excl "APPEND_ASSOC"]
 
 val ifSolves = fn x => TRY (x \\ NO_TAC)
 val ifHypx   = fn pat => (fn tac => TRY $ qpat_x_assum pat tac)
-val ifHyp    = fn pat => (fn tac => TRY $ qpat_assum pat tac)
+val ifHyp    = fn pat => (fn tac => TRY $ qpat_assum   pat tac)
 (***************************)
 (*                         *)
 (*     byte-y Theorems     *)
 (*                         *)
 (***************************)
 
+(**********************)
+(*   non-empty thms   *)
+(**********************)
 
 Theorem enc_numI_nEmp_nTermB:
   ∀x encx.
     enc_numI x = SOME encx ⇒
     ∃b bs. append encx = b::bs ∧ b ≠ endB ∧ b ≠ elseB
 Proof
-  rw[Once enc_numI_def, AllCaseEqs()] >> simp[]
+     rw[Once enc_numI_def, AllCaseEqs()]
+  >> simp[]
 QED
 
 Theorem enc_paraI_nEmp_nTermB:
@@ -65,6 +69,7 @@ Theorem enc_instr_nEmp_nTermB:
 Proof
      Cases
   >> rw[Once enc_instr_def, AllCaseEqs()]
+  >> simp[] (* will this speed up the proof? *)
   >> imp_res_tac enc_numI_nEmp_nTermB
   >> imp_res_tac enc_paraI_nEmp_nTermB
   >> imp_res_tac enc_varI_nEmp_nTermB
@@ -73,10 +78,69 @@ Proof
   >> simp[]
 QED
 
-Theorem num_cf_instr_disjoint:
+
+
+Theorem enc_valtype_nEmp_n0x40:
+  ∀x encx.
+    enc_valtype x = SOME encx ⇒
+    ∃b bs. append encx = b::bs ∧ b ≠ 0x40w
+Proof
+     namedCases ["bvtype width"]
+  \\ Cases_on ‘width’
+  >> rw[enc_valtype_def, AllCaseEqs(), bvtype_nchotomy]
+QED
+
+Theorem enc_u32_nNUL:
+  ∀x encx.
+    enc_u32 x = SOME encx ⇒ ¬NULL (append encx)
+Proof
+     simp[enc_u32_def, enc_unsigned_word_def]
+  \\ rw[Once enc_num_def]
+QED
+
+Theorem enc_vector_nEmp:
+  ∀enc xs encxs.
+    enc_vector enc xs = SOME encxs ⇒
+    ∃b bs. append encxs = b::bs
+Proof
+     Cases_on ‘xs’
+  >- simp[enc_vector_def, enc_list_def, enc_u32_def, enc_unsigned_word_def, Once enc_num_def]
+  \\ simp[enc_vector_def]
+  \\ rpt strip_tac
+  \\ imp_res_tac enc_u32_nNUL
+  \\ Cases_on ‘append encln’
+  \\ gvs[]
+QED
+
+Theorem enc_section_nEmp__nNUL:
+  ∀lb enc x xs exxs.
+    enc_section lb enc (x::xs) = SOME exxs ⇒ ¬NULL (append exxs)
+Proof
+     rw[enc_section_def]
+  \\ simp[]
+QED
+
+Theorem enc_section_nNUL__nNUL:
+  ∀lb enc xs exs.
+    ¬NULL xs ∧ enc_section lb enc xs = SOME exs ⇒
+    ¬NULL (append exs)
+Proof
+     rw[enc_section_def]
+  \\ simp[]
+QED
+
+
+
+
+
+(*********************)
+(*   disjoint thms   *)
+(*********************)
+
+Theorem num_cf_disjoint:
   ∀x encx b bs.
-    enc_numI x = SOME encx ⇒
-    append encx = b::bs ⇒
+    enc_numI x = SOME encx ∧ append encx = b::bs
+    ⇒
     b ≠ unrOC ∧ b ≠ nopOC ∧ b ≠ blkOC ∧
     b ≠ lopOC ∧ b ≠ if_OC ∧ b ≠ br_OC ∧
     b ≠ briOC ∧ b ≠ brtOC ∧ b ≠ retOC ∧
@@ -88,10 +152,10 @@ Proof
   >> gvs[]
 QED
 
-Theorem para_cf_instr_disjoint:
+Theorem para_cf_disjoint:
   ∀x encx b bs.
-    enc_paraI x = SOME encx ⇒
-    append encx = b::bs ⇒
+    enc_paraI x = SOME encx ∧ append encx = b::bs
+    ⇒
     b ≠ unrOC ∧ b ≠ nopOC ∧ b ≠ blkOC ∧
     b ≠ lopOC ∧ b ≠ if_OC ∧ b ≠ br_OC ∧
     b ≠ briOC ∧ b ≠ brtOC ∧ b ≠ retOC ∧
@@ -101,10 +165,10 @@ Proof
   Cases \\ simp[enc_paraI_def, AllCaseEqs()]
 QED
 
-Theorem var_cf_instr_disjoint:
+Theorem var_cf_disjoint:
   ∀x encx b bs.
-    enc_varI x = SOME encx ⇒
-    append encx = b::bs ⇒
+    enc_varI x = SOME encx ∧ append encx = b::bs
+    ⇒
     b ≠ unrOC ∧ b ≠ nopOC ∧ b ≠ blkOC ∧
     b ≠ lopOC ∧ b ≠ if_OC ∧ b ≠ br_OC ∧
     b ≠ briOC ∧ b ≠ brtOC ∧ b ≠ retOC ∧
@@ -116,10 +180,10 @@ Proof
   >> gvs[]
 QED
 
-Theorem load_cf_instr_disjoint:
+Theorem load_cf_disjoint:
   ∀x encx b bs.
-    enc_loadI x = SOME encx ⇒
-    append encx = b::bs ⇒
+    enc_loadI x = SOME encx ∧ append encx = b::bs
+    ⇒
     b ≠ unrOC ∧ b ≠ nopOC ∧ b ≠ blkOC ∧
     b ≠ lopOC ∧ b ≠ if_OC ∧ b ≠ br_OC ∧
     b ≠ briOC ∧ b ≠ brtOC ∧ b ≠ retOC ∧
@@ -131,10 +195,10 @@ Proof
   >> gvs[]
 QED
 
-Theorem store_cf_instr_disjoint:
+Theorem store_cf_disjoint:
   ∀x encx b bs.
-    enc_storeI x = SOME encx ⇒
-    append encx = b::bs ⇒
+    enc_storeI x = SOME encx ∧ append encx = b::bs
+    ⇒
     b ≠ unrOC ∧ b ≠ nopOC ∧ b ≠ blkOC ∧
     b ≠ lopOC ∧ b ≠ if_OC ∧ b ≠ br_OC ∧
     b ≠ briOC ∧ b ≠ brtOC ∧ b ≠ retOC ∧
@@ -146,81 +210,7 @@ Proof
   >> gvs[]
 QED
 
-Theorem var_para_disjoint:
-  ∀x encx rest.
-    enc_paraI x = SOME encx ⇒
-    ∃e. dec_varI (encx a++ rest) = (INL e, append encx ++ rest)
-Proof
-  Cases
-  >> rw[enc_paraI_def, AllCaseEqs(), Once dec_varI_def]
-  >> Cases_on ‘dec_u32 rest’
-  >> Cases_on ‘q’
-  >> simp[]
-QED
 
-Theorem var_num_disjoint:
-  ∀x encx rest.
-    enc_numI x = SOME encx ⇒
-    ∃e. dec_varI (encx a++ rest) = (INL e, append encx ++ rest)
-Proof
-  rw[]
-  \\ imp_res_tac enc_numI_nEmp_nTermB
-  \\ gvs[dec_varI_def, AllCaseEqs()]
-  \\ Cases_on ‘dec_u32 (bs ++ rest)’
-  \\ Cases_on ‘q’
-  >> simp[]
-    \\ last_x_assum mp_tac
-    \\ rw[enc_numI_def, AllCaseEqs()]
-    >> gvs[]
-QED
-
-Theorem para_num_disjoint:
-  ∀x encx rest.
-    enc_numI x = SOME encx ⇒
-    ∃e. dec_paraI (encx a++ rest) = (INL e, append encx ++ rest)
-Proof
-  Cases >> gen_tac
-  >> rw[enc_numI_def, AllCaseEqs()]
-  >> simp[dec_paraI_def]
-QED
-
-Theorem var_load_disjoint:
-  ∀x encx rest.
-    enc_loadI x = SOME encx ⇒
-    ∃e. dec_varI (append encx ++ rest) = (INL e, append encx ++ rest)
-Proof
-  rw[]
-  \\ imp_res_tac enc_loadI_nEmp_nTermB
-  \\ gvs[dec_varI_def, AllCaseEqs()]
-  \\ Cases_on ‘dec_u32 (bs ++ rest)’
-  \\ Cases_on ‘q’
-  >> simp[]
-    \\ last_x_assum mp_tac
-    \\ rw[enc_loadI_def, AllCaseEqs()]
-    >> gvs[]
-QED
-
-Theorem para_load_disjoint:
-  ∀x encx rest.
-    enc_loadI x = SOME encx ⇒
-    ∃e. dec_paraI (append encx ++ rest) = (INL e, append encx ++ rest)
-Proof
-  Cases >> gen_tac
-  >> simp[enc_loadI_def, AllCaseEqs()]
-  >> rpt strip_tac
-  >> gvs[dec_paraI_def]
-QED
-
-Theorem num_load_disjoint:
-  ∀x encx rest.
-    enc_loadI x = SOME encx ⇒
-    ∃e. dec_numI (append encx ++ rest) = (INL e, append encx ++ rest)
-Proof
-  Cases >> gen_tac
-  >> simp[enc_loadI_def, AllCaseEqs()]
-  >> rpt strip_tac
-  >> gvs[dec_numI_def]
-QED
 
 Theorem var_store_disjoint:
   ∀x encx rest.
@@ -270,56 +260,94 @@ Proof
   >> gvs[dec_loadI_def]
 QED
 
-Theorem enc_valtype_nEmp_n0x40:
-  ∀x encx.
-    enc_valtype x = SOME encx ⇒
-    ∃b bs. append encx = b::bs ∧ b ≠ 0x40w
+
+
+Theorem var_load_disjoint:
+  ∀x encx rest.
+    enc_loadI x = SOME encx ⇒
+    ∃e. dec_varI (append encx ++ rest) = (INL e, append encx ++ rest)
 Proof
-  Cases
-  >> Cases_on ‘w’
-  >> rw[enc_valtype_def, AllCaseEqs(), bvtype_nchotomy]
-QED
-
-
-
-Theorem enc_u32_nEmp:
-  ∀x encx.
-    enc_u32 x = SOME encx ⇒ ¬NULL (append encx)
-Proof
-     simp[enc_u32_def, enc_unsigned_word_def]
-  \\ rw[Once enc_num_def]
-QED
-
-Theorem enc_vector_nEmp:
-  ∀enc xs encxs.
-    enc_vector enc xs = SOME encxs ⇒
-    ∃b bs. append encxs = b::bs
-Proof
-     Cases_on ‘xs’
-  >- simp[enc_vector_def, enc_list_def, enc_u32_def, enc_unsigned_word_def, Once enc_num_def]
-  \\ simp[enc_vector_def]
-  \\ rpt strip_tac
-  \\ imp_res_tac enc_u32_nEmp
-  \\ Cases_on ‘append encln’
-  \\ gvs[]
-QED
-
-Theorem enc_section_nEmp:
-  ∀lb enc x xs exxs.
-    enc_section lb enc (x::xs) = SOME exxs ⇒ ¬NULL (append exxs)
-Proof
-     rw[enc_section_def]
-  \\ simp[]
-QED
-
-Theorem enc_section_nEmp':
-  ∀lb enc xs exs.
-    ¬NULL xs ∧ enc_section lb enc xs = SOME exs ⇒
-    ¬NULL (append exs)
-Proof
-     rw[enc_section_def]
+     rw[]
+  \\ imp_res_tac enc_loadI_nEmp_nTermB
+  \\ gvs[dec_varI_def, AllCaseEqs()]
+  \\ Cases_on ‘dec_u32 (bs ++ rest)’
+  \\ Cases_on ‘q’
   >> simp[]
+    \\ last_x_assum mp_tac
+    \\ rw[enc_loadI_def, AllCaseEqs()]
+    >> gvs[]
 QED
+
+Theorem para_load_disjoint:
+  ∀x encx rest.
+    enc_loadI x = SOME encx ⇒
+    ∃e. dec_paraI (append encx ++ rest) = (INL e, append encx ++ rest)
+Proof
+  Cases >> gen_tac
+  >> simp[enc_loadI_def, AllCaseEqs()]
+  >> rpt strip_tac
+  >> gvs[dec_paraI_def]
+QED
+
+Theorem num_load_disjoint:
+  ∀x encx rest.
+    enc_loadI x = SOME encx ⇒
+    ∃e. dec_numI (append encx ++ rest) = (INL e, append encx ++ rest)
+Proof
+  Cases >> gen_tac
+  >> simp[enc_loadI_def, AllCaseEqs()]
+  >> rpt strip_tac
+  >> gvs[dec_numI_def]
+QED
+
+
+
+Theorem var_num_disjoint:
+  ∀x encx rest.
+    enc_numI x = SOME encx ⇒
+    ∃e. dec_varI (encx a++ rest) = (INL e, append encx ++ rest)
+Proof
+     rw[]
+  \\ imp_res_tac enc_numI_nEmp_nTermB
+  \\ gvs[dec_varI_def, AllCaseEqs()]
+  \\ namedCases_on ‘dec_u32 (bs ++ rest)’ ["either rs"]
+  \\ namedCases_on ‘either’ ["e", "x"]
+  >> simp[]
+    \\ last_x_assum mp_tac
+    \\ rw[enc_numI_def, AllCaseEqs()]
+    >> gvs[]
+QED
+
+Theorem para_num_disjoint:
+  ∀x encx rest.
+    enc_numI x = SOME encx ⇒
+    ∃e. dec_paraI (encx a++ rest) = (INL e, append encx ++ rest)
+Proof
+     Cases
+  >> gen_tac
+    >> rw[enc_numI_def, AllCaseEqs()]
+    >> simp[dec_paraI_def]
+QED
+
+
+
+Theorem var_para_disjoint:
+  ∀x encx rest.
+    enc_paraI x = SOME encx ⇒
+    ∃e. dec_varI (encx a++ rest) = (INL e, append encx ++ rest)
+Proof
+     Cases
+  >> rw[enc_paraI_def, AllCaseEqs(), Once dec_varI_def]
+    >> namedCases_on ‘dec_u32 rest’ ["either rs"]
+    >> namedCases_on ‘either’ ["e", "x"]
+    >> simp[]
+QED
+
+
+
+
+
+
 
 
 (***********************************)
@@ -338,19 +366,17 @@ fun print_dot_tac h = (print "."; all_tac h);
 Theorem dec_enc_vector:
   ∀enc dec is encis.
     enc_vector enc is = SOME encis ∧
-    (∀x encx rs. enc x = SOME encx ⇒ dec (append encx ++ rs) = (INR x,rs))
+    (∀rs x encx. enc x = SOME encx ⇒ dec (append encx ++ rs) = (INR x,rs))
     ⇒
     ∀rest. dec_vector dec (encis a++ rest) = (INR is, rest)
 Proof
-  rpt strip_tac
+     rpt strip_tac
   \\ last_x_assum mp_tac
-  \\ simp[dec_vector_def, enc_vector_def, AllCaseEqs(), GSYM NOT_LESS]
-  \\ rpt strip_tac
+  \\ rw[enc_vector_def, dec_vector_def, AllCaseEqs()]
   \\ gvs ssa
   \\ imp_res_tac dec_enc_u32
   \\ simp[]
-  \\ (* tidy up from dec enc vec pf *)
-     ntac 2 $ pop_assum kall_tac
+  \\ ntac 2 $ pop_assum kall_tac (* tidy up from dec enc vec pf *)
   (* dec_enc_list *)
   \\ pop_assum mp_tac
   \\ qid_spec_tac ‘rest’
@@ -370,24 +396,24 @@ QED
 (*************)
 
 Theorem dec_enc_valtype:
-  ∀x encx rest.
+  ∀rest x encx.
     enc_valtype x = SOME encx ⇒
     dec_valtype (encx a++ rest) = (INR x, rest)
 Proof
-     Cases
+     namedCases_on ‘x’ ["bvtype width"]
   \\ simp[bvtype_nchotomy, enc_valtype_def, dec_valtype_def, AllCaseEqs()]
-  \\ Cases_on ‘w’
+  \\ Cases_on ‘width’
   >> simp[]
 QED
 
 Theorem dec_enc_functype:
-  ∀x encx rest.
+  ∀rest x encx.
     enc_functype x = SOME encx ⇒
     dec_functype (encx a++ rest) = (INR x, rest)
 Proof
-     rw[enc_functype_def, AllCaseEqs()]
-  \\ PairCases_on ‘x’
-  \\ gvs[dec_functype_def, AllCaseEqs()]
+     namedCases_on ‘x’ ["args retvs"]
+  \\ rw[enc_functype_def, AllCaseEqs()]
+  \\ simp[dec_functype_def, AllCaseEqs()]
   \\ rpt $ dxrule dec_enc_vector
   \\ rpt $ disch_then $ qspec_then ‘dec_valtype’ assume_tac
   \\ gvs[dec_enc_valtype]
@@ -395,7 +421,7 @@ Proof
 QED
 
 Theorem dec_enc_limits:
-  ∀x encx rest.
+  ∀rest x encx.
     enc_limits x = SOME encx ⇒
     dec_limits (encx a++ rest) = (INR x, rest)
 Proof
@@ -404,7 +430,7 @@ Proof
 QED
 
 Theorem dec_enc_globaltype:
-  ∀x encx rest.
+  ∀rest x encx.
     enc_globaltype x = SOME encx ⇒
     dec_globaltype (encx a++ rest) = (INR x, rest)
 Proof
@@ -414,14 +440,14 @@ QED
 
 
 
-(*******************************************)
-(*   Instructions (hierarchically lower)   *)
-(*******************************************)
+(******************************************************)
+(*   Instructions (hierarchically lower components)   *)
+(******************************************************)
 
 Theorem dec_enc_numI:
-  ∀x encx.
+  ∀rest x encx.
     enc_numI x = SOME encx ⇒
-    ∀rest. dec_numI (encx a++ rest) = (INR x, rest)
+    dec_numI (encx a++ rest) = (INR x, rest)
 Proof
      rw[enc_numI_def, AllCaseEqs(), bvtype_nchotomy, convert_op_nchotomy]
   >> simp[]
@@ -432,37 +458,37 @@ Proof
 QED
 
 Theorem dec_enc_paraI:
-  ∀x encx.
+  ∀rest x encx.
     enc_paraI x = SOME encx ⇒
-    ∀rest. dec_paraI (encx a++ rest) = (INR x, rest)
+    dec_paraI (encx a++ rest) = (INR x, rest)
 Proof
-     Cases
+     Cases_on ‘x’
   >> rw[enc_paraI_def, AllCaseEqs()]
   >> simp[dec_paraI_def]
 QED
 
 Theorem dec_enc_varI:
-  ∀x encx.
+  ∀rest x encx.
     enc_varI x = SOME encx ⇒
-    ∀rest. dec_varI (encx a++ rest) = (INR x, rest)
+    dec_varI (encx a++ rest) = (INR x, rest)
 Proof
      rw[enc_varI_def, AllCaseEqs()]
   >> simp[dec_varI_def, AllCaseEqs(), dec_enc_u32]
 QED
 
 Theorem dec_enc_loadI:
-  ∀x encx.
+  ∀rest x encx.
     enc_loadI x = SOME encx ⇒
-    ∀rest. dec_loadI (encx a++ rest) = (INR x, rest)
+    dec_loadI (encx a++ rest) = (INR x, rest)
 Proof
      rw[enc_loadI_def, AllCaseEqs(), bvtype_nchotomy]
   >> simp[dec_loadI_def, AllCaseEqs(), dec_enc_2u32]
 QED
 
 Theorem dec_enc_storeI:
-  ∀x encx.
+  ∀rest x encx.
     enc_storeI x = SOME encx ⇒
-    ∀rest. dec_storeI (encx a++ rest) = (INR x, rest)
+    dec_storeI (encx a++ rest) = (INR x, rest)
 Proof
      rw[enc_storeI_def, AllCaseEqs(), bvtype_nchotomy]
   >> simp[dec_storeI_def, AllCaseEqs(), dec_enc_2u32]
@@ -477,24 +503,23 @@ QED
 (**********************************************)
 
 Theorem dec_enc_blocktype:
-  ∀x encx.
+  ∀rest x encx.
     enc_blocktype x = SOME encx ⇒
-    ∀rest. dec_blocktype (encx a++ rest) = (INR x, rest)
+    dec_blocktype (encx a++ rest) = (INR x, rest)
 Proof
-  rw[enc_blocktype_def, AllCaseEqs()]
+     rw[enc_blocktype_def, AllCaseEqs()]
   >> simp[dec_blocktype_def, AllCaseEqs()]
   \\ imp_res_tac enc_valtype_nEmp_n0x40
   \\ imp_res_tac dec_enc_valtype
   \\ gvs[]
 QED
 
-
 Theorem dec_enc_indxs:
-  ∀x encx.
+  ∀rest x encx.
   enc_indxs x = SOME encx ⇒
-  ∀rest. dec_indxs (encx a++ rest) = (INR x, rest)
+  dec_indxs (encx a++ rest) = (INR x, rest)
 Proof
-  rpt strip_tac
+     rpt strip_tac
   \\ qspec_then ‘enc_u32’ irule dec_enc_vector
   \\ assume_tac dec_enc_u32
   \\ simp[]
@@ -542,7 +567,7 @@ Proof (* Note - all the work is really done in the instr (VS instr_list) case *)
   (**)
   >>~- ([‘enc_numI’  ],
          imp_res_tac enc_numI_nEmp_nTermB
-      \\ imp_res_tac num_cf_instr_disjoint
+      \\ imp_res_tac num_cf_disjoint
       \\ imp_res_tac para_num_disjoint
       \\ imp_res_tac var_num_disjoint
       \\ rpt $ pop_assum $ qspec_then ‘rs’ mp_tac
@@ -555,7 +580,7 @@ Proof (* Note - all the work is really done in the instr (VS instr_list) case *)
   )
   >>~- ([‘enc_paraI’ ],
          imp_res_tac enc_paraI_nEmp_nTermB
-      \\ imp_res_tac para_cf_instr_disjoint
+      \\ imp_res_tac para_cf_disjoint
       \\ imp_res_tac var_para_disjoint
       \\ pop_assum $ qspec_then ‘rs’ strip_assume_tac
       \\ gvs[Once dec_instr_def, AllCaseEqs()]
@@ -566,7 +591,7 @@ Proof (* Note - all the work is really done in the instr (VS instr_list) case *)
   )
   >>~- ([‘enc_varI’  ],
          imp_res_tac enc_varI_nEmp_nTermB
-      \\ imp_res_tac var_cf_instr_disjoint
+      \\ imp_res_tac var_cf_disjoint
       \\ gvs[Once dec_instr_def, AllCaseEqs()]
       (**)
       \\ ‘b::(bs ++ rs) = append encx ++ rs’ by simp[]
@@ -575,7 +600,7 @@ Proof (* Note - all the work is really done in the instr (VS instr_list) case *)
   )
   >>~- ([‘enc_loadI’ ],
          imp_res_tac enc_loadI_nEmp_nTermB
-      \\ imp_res_tac load_cf_instr_disjoint
+      \\ imp_res_tac load_cf_disjoint
       \\ imp_res_tac var_load_disjoint
       \\ imp_res_tac para_load_disjoint
       \\ imp_res_tac num_load_disjoint
@@ -589,7 +614,7 @@ Proof (* Note - all the work is really done in the instr (VS instr_list) case *)
   )
   >>~- ([‘enc_storeI’],
          imp_res_tac enc_storeI_nEmp_nTermB
-      \\ imp_res_tac store_cf_instr_disjoint
+      \\ imp_res_tac store_cf_disjoint
       \\ imp_res_tac var_store_disjoint
       \\ imp_res_tac para_store_disjoint
       \\ imp_res_tac num_store_disjoint
@@ -610,19 +635,21 @@ Proof (* Note - all the work is really done in the instr (VS instr_list) case *)
 QED
 
 Triviality dec_enc_instr_list:
-  ∀e is dc encis rest.
+  ∀rest e is dc encis.
     enc_instr_list e is = SOME encis ⇒
     dec_instr_list (¬e ∨ dc) (encis a++ rest) = ret rest (exprB e,is)
 Proof
-  strip_assume_tac dec_enc_instructions
+     rpt gen_tac
+  \\ rw[dec_enc_instructions]
 QED
 
 Triviality dec_enc_instr:
-  ∀i enci rest.
+  ∀rest i enci.
     enc_instr i = SOME enci ⇒
     dec_instr $ enci a++ rest = ret rest i
 Proof
-  strip_assume_tac dec_enc_instructions
+     rpt gen_tac
+  \\ rw[dec_enc_instructions]
 QED
 
 Triviality dec_enc_expr:
@@ -630,9 +657,9 @@ Triviality dec_enc_expr:
     enc_expr is = SOME encis ⇒
     dec_instr_list dc (encis a++ rest) = ret rest (endB,is)
 Proof
-     rw[]
+     rpt strip_tac
   \\ dxrule dec_enc_instr_list
-  \\ rw[]
+  \\ simp[]
 QED
 
 Triviality dec_enc_tArm:
@@ -664,8 +691,7 @@ Proof
 QED
 
 Triviality s2b_b2s__I[simp]:
-  ∀x.
-  string2bytes $ bytes2string x = x
+  ∀x. string2bytes $ bytes2string x = x
 Proof
   rw[string2bytes_def, bytes2string_def, MAP_MAP_o, n2w_ORD_CHR_w2n, MAP_ID_I]
 QED
@@ -677,10 +703,15 @@ Proof
 QED
 
 Triviality b2s_s2b__I[simp]:
-  ∀x.
-  bytes2string $ string2bytes x = x
+  ∀x. bytes2string $ string2bytes x = x
 Proof
   rw[string2bytes_def, bytes2string_def, MAP_MAP_o, CHR_w2n_n2w_ORD, MAP_ID_I]
+QED
+
+Triviality imp_b2s_null:
+  ∀x. bytes2string x = "" ⇒ x = []
+Proof
+  simp[implode_def, bytes2string_def]
 QED
 
 Triviality imp_b2s_null[simp]:
@@ -695,12 +726,17 @@ Proof
   simp[implode_def]
 QED
 
-Triviality s2b_explode[simp]:
-  ∀x.
-  string2bytes (explode x) = [] ⇔ x = «»
+Triviality id_OK_emp[simp]:
+  id_OK ""
 Proof
-  gen_tac
-  \\ simp[string2bytes_def]
+  simp[id_OK_def]
+QED
+
+Triviality s2b_explode_NUL:
+  ∀x. NULL (string2bytes (explode x)) ⇔ x = «»
+Proof
+     gen_tac
+  \\ simp[string2bytes_def, NULL_EQ_NIL]
   \\ iff_tac
   >> rw[]
   \\ qspec_then ‘x’ mp_tac implode_explode
@@ -716,89 +752,105 @@ Proof
 QED
 
 Triviality b2s__STRING[simp]:
-  ∀s' ss.
-  implode (bytes2string (n2w (ORD s')::MAP (n2w ∘ ORD) ss)) = implode $ STRING s' ss
+  ∀s' ss. implode (bytes2string (n2w (ORD s')::MAP (n2w ∘ ORD) ss)) = implode $ STRING s' ss
 Proof
   rw[bytes2string_def, MAP_MAP_o, CHR_w2n_n2w_ORD]
 QED
 
 
-Theorem enc_section_empty[simp]:
-  ∀lb enc.
-  enc_section lb enc [] = SOME $ List []
+
+
+
+Theorem enc_section_emp[simp]:
+  ∀lb enc. enc_section lb enc [] = SOME $ List []
 Proof
   rw[enc_section_def]
 QED
 
-Theorem enc_section_empty_conv:
+Theorem enc_section_emp__NUL_conv:
   ∀lb enc xs encxs.
-  NULL (append encxs) ∧
-  enc_section lb enc xs = SOME encxs ⇒ xs = []
+    enc_section lb enc xs = SOME encxs ∧ NULL (append encxs) ⇒ xs = []
 Proof
-     rw[enc_section_def, NULL_EQ_NIL, prepend_sz_def]
-  >> gvs[append_def]
+     rw[enc_section_def, NULL_EQ_NIL, prepend_B_sz_def]
+  \\ gvs[append_def]
 QED
-
 
 Triviality enc_names_section_blank[simp]:
   enc_names_section blank_names = SOME $ List []
 Proof
      rw[enc_names_section_def, blank_names_def, enc_section_def]
-  >> fs[id_OK_def, prepend_sz_def, enc_u32_def, magic_bytes_def, string2bytes_def]
+  >- simp[prepend_B_sz_def, name_bytes_def, string2bytes_def, enc_u32_def]
+  >- fs[string2bytes_def]
 QED
 
-Triviality enc_names_section_blank_conv:
-  ∀x ex.
-  enc_names_section x = SOME ex ∧ NULL (append ex) ⇒
-  x = blank_names
+Triviality enc_names_section_blank__NUL_conv:
+  ∀x ex. enc_names_section x = SOME ex ∧ NULL (append ex) ⇒ x = blank_names
 Proof
-     rw[enc_names_section_def, enc_section_def, NULL_EQ_NIL, blank_names_values]
-  >> Cases_on ‘x’
-  >> gvs[names_component_equality]
+(* askyk askmm *)
+     namedCases_on ‘x’ ["mname fnames lnames"]
+  \\ rw[enc_names_section_def, blank_names_values]
+  >-(
+       Cases_on ‘NULL $ string2bytes $ explode mname’
+    >- imp_res_tac s2b_explode_NUL
+    \\ imp_res_tac enc_section_nNUL__nNUL
+    \\ ntac 2 $ pop_assum kall_tac
+    \\ gvs[]
+  )
+  >-(
+       Cases_on ‘NULL fnames’
+    >- gvs[NULL_EQ_NIL]
+    \\ imp_res_tac enc_section_nNUL__nNUL
+    \\ ntac 2 $ pop_assum kall_tac
+    \\ gvs[]
+  )
+  \\ Cases_on ‘NULL lnames’
+  >- gvs[NULL_EQ_NIL]
+  \\ imp_res_tac enc_section_nNUL__nNUL
+  \\ ntac 2 $ pop_assum kall_tac
+  \\ gvs[]
 QED
 
 Triviality names_not_blank:
-  ∀x.
-  x ≠ blank_names ⇒ x.mname ≠ «» ∨ ¬NULL x.fnames ∨ ¬NULL x.lnames
+  ∀x. x ≠ blank_names ⇒ x.mname ≠ «» ∨ ¬NULL x.fnames ∨ ¬NULL x.lnames
 Proof
-     namedCases ["m_name f_names l_names"]
-  \\ namedCases_on ‘m_name’ ["s"]
+     namedCases ["mname fnames lnames"]
+  \\ namedCases_on ‘mname’ ["x"]
   \\ rewrite_tac[GSYM implode_def]
-  \\ namedCases_on ‘s’ ["", "s ss"]
-  >> namedCases_on ‘f_names’ ["", "f fs"]
-  >> namedCases_on ‘l_names’ ["", "l ls"]
+  \\ namedCases_on ‘x’ ["", "s ss"]
+  >> namedCases_on ‘fnames’ ["", "f fs"]
+  >> namedCases_on ‘lnames’ ["", "l ls"]
   >> simp[blank_names_values]
 QED
 
 Triviality names_not_blank':
-  ∀x.
-  x ≠ blank_names ⇒ ¬NULL (string2bytes $ explode x.mname) ∨ ¬NULL x.fnames ∨ ¬NULL x.lnames
+  ∀x. x ≠ blank_names ⇒ ¬NULL (string2bytes $ explode x.mname) ∨ ¬NULL x.fnames ∨ ¬NULL x.lnames
 Proof
-     ntac 2 $ rpt strip_tac
+     rpt strip_tac
   \\ imp_res_tac names_not_blank
   >> simp[]
-  \\ Cases_on ‘x.mname’
-  \\ Cases_on ‘s’
+  \\ namedCases_on ‘x.mname’ ["s"]
+  \\ namedCases_on ‘s’ ["", "s ss"]
   >> gvs[string2bytes_def]
 QED
 
 
-Triviality enc_names_section_nEmp:
+
+Triviality enc_names_section_not_blank__nNUL:
   ∀x encx.
-  x ≠ blank_names ∧ enc_names_section x = SOME encx ⇒
-  ¬NULL (append encx)
+    x ≠ blank_names ∧ enc_names_section x = SOME encx ⇒
+    ¬NULL (append encx)
 Proof
      rpt strip_tac
-  \\ imp_res_tac enc_names_section_blank_conv
+  \\ imp_res_tac enc_names_section_blank__NUL_conv
 QED
 
-Triviality enc_names_section_nEmp':
+Triviality enc_names_section_not_blank__lbn0:
   ∀x encx.
     x ≠ blank_names ∧ enc_names_section x = SOME encx ⇒
     ∃dc. append encx = 0w::dc
 Proof
      rpt strip_tac
-  \\ drule enc_names_section_blank_conv
+  \\ drule enc_names_section_blank__NUL_conv
   \\ rw[]
   \\ gvs[oneline enc_names_section_def, NULL_EQ_NIL]
   >> Cases_on ‘append ss0’
@@ -806,6 +858,9 @@ Proof
   >> Cases_on ‘append ss2’
   >> gvs[]
 QED
+
+
+
 
 
 Triviality dec_names_section_empty[simp]:
@@ -828,13 +883,16 @@ QED
 
 
 
-Theorem dec_enc_global[simp]:
-  ∀g encg rest.
+Theorem dec_enc_global:
+  ∀rest g encg.
     enc_global g = SOME encg ⇒
     dec_global $ encg a++ rest = (INR g, rest)
 Proof
      rw $ ssaa [enc_global_def, dec_global_def, AllCaseEqs()]
-  >-( Cases_on ‘g.gtype’ >> gvs[enc_globaltype_def] )
+  >-(
+       Cases_on ‘g.gtype’
+    >> gvs[enc_globaltype_def]
+  )
   \\ imp_res_tac dec_enc_globaltype
   \\ imp_res_tac dec_enc_instr_list
   \\ pop_assum $ qspecl_then [‘rest’, ‘F’] assume_tac
@@ -845,13 +903,16 @@ QED
 
 
 Theorem dec_enc_code:
-  ∀cd encC rs.
+  ∀rest cd encC.
     enc_code cd = SOME encC ⇒
-    dec_code $ encC a++ rs = (INR cd, rs)
+    dec_code $ encC a++ rest = (INR cd, rest)
 Proof
-  PairCases
-  \\ rw[enc_code_def, AllCaseEqs(), dec_code_def, prepend_sz_def]
-  >-( imp_res_tac enc_u32_nEmp \\ simp[] )
+     namedCases_on `cd` ["argTs exp"]
+  \\ rw[enc_code_def, AllCaseEqs(), dec_code_def, prepend_B_sz_def]
+  >-(
+       imp_res_tac enc_u32_nNUL
+    \\ simp[]
+  )
   \\ simp ssa
   \\ imp_res_tac dec_enc_u32
   \\ gvs[]
@@ -865,7 +926,7 @@ QED
 
 
 Theorem dec_enc_byte:
-  ∀x encx rest.
+  ∀rest x encx.
     enc_byte x = SOME encx ⇒
     dec_byte $ encx a++ rest = (INR x, rest)
 Proof
@@ -875,45 +936,45 @@ QED
 
 
 Theorem dec_enc_data:
-  ∀dt encD rs.
+  ∀rest dt encD.
     enc_data dt = SOME encD ⇒
-    dec_data $ encD a++ rs = (INR dt, rs)
+    dec_data $ encD a++ rest = (INR dt, rest)
 Proof
      rw[enc_data_def, dec_data_def, AllCaseEqs()]
-  >> imp_res_tac enc_u32_nEmp
+  >> imp_res_tac enc_u32_nNUL
   >> simp ssa
   \\ imp_res_tac dec_enc_u32
   \\ simp[]
   \\ dxrule_at Any dec_enc_instr_list
   \\ rw ssa
-  \\ ntac 3 $ pop_assum kall_tac
   \\ assume_tac dec_enc_byte
   \\ imp_res_tac dec_enc_vector
   \\ simp[data_component_equality]
 QED
 
 
+
 Theorem dec_enc_mls:
-  ∀x encx rest.
+  ∀rest x encx.
     enc_mls x = SOME encx ⇒
     dec_mls $ encx a++ rest = (INR x, rest)
 Proof
-  rw[dec_mls_def, enc_mls_def]
+     rw[dec_mls_def, enc_mls_def]
   \\ assume_tac dec_enc_byte
   \\ imp_res_tac dec_enc_vector
   \\ simp[string2bytes_def, bytes2string_def, MAP_MAP_o, CHR_w2n_n2w_ORD]
 QED
 
 Theorem dec_enc_idx_alpha:
-  ∀enc dec x encx rest.
+  ∀rest enc dec x encx.
     enc_idx_alpha enc x = SOME encx ∧
-    (∀y ency rs. enc y = SOME ency ⇒ dec (append ency ++ rs) = (INR y,rs))
+    (∀rs y ency. enc y = SOME ency ⇒ dec (append ency ++ rs) = (INR y,rs))
     ⇒
     dec_idx_alpha dec $ encx a++ rest = (INR x, rest)
 Proof
-  rpt strip_tac
+     rpt strip_tac
   \\ last_x_assum mp_tac
-  \\ PairCases_on ‘x’
+  \\ namedCases_on ‘x’ ["idx alpha"]
   \\ simp[dec_idx_alpha_def, enc_idx_alpha_def, AllCaseEqs()]
   \\ rpt strip_tac
   \\ gvs ssa
@@ -922,37 +983,39 @@ Proof
 QED
 
 Theorem dec_enc_ass:
-  ∀x encx rest.
+  ∀rest x encx.
     enc_ass x = SOME encx ⇒
     dec_ass $ encx a++ rest = (INR x, rest)
 Proof
-  rw[dec_ass_def, enc_ass_def]
+     rw[dec_ass_def, enc_ass_def]
   \\ assume_tac dec_enc_mls
   \\ imp_res_tac dec_enc_idx_alpha
   \\ simp[]
 QED
 
 Theorem dec_enc_map:
-  ∀x encx rest.
+  ∀rest x encx.
     enc_map x = SOME encx ⇒
     dec_map $ encx a++ rest = (INR x, rest)
 Proof
-  rw[dec_map_def, enc_map_def]
+     rw[dec_map_def, enc_map_def]
   \\ assume_tac dec_enc_ass
   \\ imp_res_tac dec_enc_vector
   \\ simp[]
 QED
 
 
+
+
+
 Theorem dec_enc_section_NE: (* non empty *)
-  ∀lb xs enc dec encxs rest.
-    ¬(NULL xs)                                                      ∧
-    enc_section lb enc xs = SOME encxs                              ∧
-    (∀x encx rs. enc x = SOME encx ⇒ dec (encx a++ rs) = (INR x, rs))
+  ∀rest lb xs enc dec encxs.
+    ¬NULL xs ∧ enc_section lb enc xs = SOME encxs ∧
+    (∀rs x encx. enc x = SOME encx ⇒ dec (encx a++ rs) = (INR x, rs))
     ⇒
     dec_section lb dec $ encxs a++ rest= (INR xs, rest)
 Proof
-     rw[enc_section_def, prepend_sz_def]
+     rw[enc_section_def, prepend_B_sz_def]
   \\ simp[dec_section_def]
   \\ imp_res_tac dec_enc_u32
   \\ simp ssa
@@ -962,66 +1025,63 @@ QED
 
 Theorem dec_enc_section_NR: (* no rest *)
   ∀lb xs enc dec encxs.
-    enc_section lb enc xs = SOME encxs                              ∧
-    (∀x encx rs. enc x = SOME encx ⇒ dec (encx a++ rs) = (INR x, rs))
+    enc_section lb enc xs = SOME encxs ∧
+    (∀rs x encx. enc x = SOME encx ⇒ dec (encx a++ rs) = (INR x, rs))
     ⇒
     dec_section lb dec $ append encxs = (INR xs, [])
 Proof
-     rw[enc_section_def, prepend_sz_def]
-  >- (Cases_on ‘xs’ >> gvs[NULL, dec_section_def])
-  \\ simp[dec_section_def]
-  \\ imp_res_tac dec_enc_u32
-  \\ simp ssa
-  \\ imp_res_tac dec_enc_vector
-  \\ pop_assum $ qspec_then ‘[]’ mp_tac
-  \\ simp[]
+     rpt strip_tac
+  \\ Cases_on ‘NULL xs’
+  >- gvs[enc_section_def, NULL_EQ_NIL]
+  \\ qspec_then ‘[]’ imp_res_tac dec_enc_section_NE
+  \\ gvs[]
 QED
 
 Theorem dec_enc_section:
-  ∀lb xs enc dec encxs rest.
-    enc_section lb enc xs = SOME encxs                              ∧
-    (∀x encx rs. enc x = SOME encx ⇒ dec (encx a++ rs) = (INR x, rs))
+  ∀rest lb xs enc dec encxs.
+    enc_section lb enc xs = SOME encxs ∧
+    (∀rs x encx. enc x = SOME encx ⇒ dec (encx a++ rs) = (INR x, rs))
     ⇒
     dec_section lb dec $ encxs a++ rest = (INR xs, rest) ∨ xs = []
 Proof
      Cases_on ‘xs’
-  >> rw[enc_section_def, prepend_sz_def]
+  >> rw[enc_section_def, prepend_B_sz_def]
   \\ imp_res_tac dec_enc_u32
   \\ imp_res_tac dec_enc_vector
   \\ simp $ ssaa [dec_section_def]
 QED
 
 
-Theorem dec_section_passThrough:
+Theorem dec_section_pt:
   ∀lb b dec bs. lb ≠ b ⇒ dec_section lb dec (b::bs) = ret (b::bs) []
 Proof
   simp[Once dec_section_def]
 QED
 
-Theorem enc_dec_section_passThrough:
+Theorem enc_dec_section_pt:
   ∀b2 dec b1 enc x xs exxs.
-    b1 ≠ b2                              ∧
+    b1 ≠ b2 ∧
     enc_section b1 enc (x::xs) = SOME exxs ⇒
     dec_section b2 dec $ append exxs = ret (append exxs) []
 Proof
      rw[enc_section_def]
-  \\ rw[dec_section_passThrough]
+  \\ rw[dec_section_pt]
 QED
 
-Theorem enc_dec_section_passThrough_rest:
+Theorem enc_dec_section_ptr:
   ∀b2 dec b1 enc rest x xs exxs.
-    b1 ≠ b2                              ∧
+    b1 ≠ b2 ∧
     enc_section b1 enc (x::xs) = SOME exxs ⇒
     dec_section b2 dec $ exxs a++ rest = ret (exxs a++ rest) []
 Proof
      rw[enc_section_def]
-  \\ rw[dec_section_passThrough]
+  \\ rw[dec_section_pt]
 QED
 
 
 
-Theorem dec_enc_names_passThrough:
-  ∀b rest. b ≠ 0w ⇒ dec_names_section $ (b::rest) = ret (b::rest) []
+Theorem dec_enc_names_pt:
+  ∀rest b. b ≠ 0w ⇒ dec_names_section $ (b::rest) = ret (b::rest) []
 Proof
   rw[Once dec_names_section_def]
 QED
@@ -1034,10 +1094,12 @@ Proof
   rw[blank_mod_def, enc_mod_and_names_def, split_funcs_def]
 QED
 
+
+
 Theorem split_zip_funcs:
   ∀fs fs_types fs_lbods.
-  split_funcs fs = (fs_types, fs_lbods) ⇒
-  zip_funcs fs_types fs_lbods = fs
+    split_funcs fs = (fs_types, fs_lbods) ⇒
+    zip_funcs fs_types fs_lbods = fs
 Proof
      Induct
   >> rw[split_funcs_def, zip_funcs_def]
@@ -1046,178 +1108,187 @@ Proof
 QED
 
 
-(**********************************************************************)
-(*   Some widgets to make the names proof more modular and abstract   *)
-(**********************************************************************)
+(*****************************************************************************)
+(*   Some widgets to make the names/module proof more modular and abstract   *)
+(*****************************************************************************)
 
-Triviality widget0_rest:
+(* dec-enc sub-section (specialized) thms. used in the names_section proof *)
+Triviality dess0r:
   ∀rest x xs ex.
     enc_section 0w enc_byte (x::xs) = SOME ex ⇒
     dec_section 0w dec_byte (ex a++ rest) = ret rest (x::xs)
 Proof
      rpt strip_tac
-  >> imp_res_tac enc_section_nEmp
-  >> assume_tac dec_enc_byte
-  >> imp_res_tac dec_enc_section
-  >> pop_assum $ qspec_then ‘rest’ mp_tac
-  >> simp[]
+  \\ imp_res_tac enc_section_nEmp__nNUL
+  \\ assume_tac dec_enc_byte
+  \\ imp_res_tac dec_enc_section
+  \\ pop_assum $ qspec_then ‘rest’ mp_tac
+  \\ simp[]
 QED
 
-Triviality widget0:
+Triviality dess0:
   ∀x xs ex.
     enc_section 0w enc_byte (x::xs) = SOME ex ⇒
     dec_section 0w dec_byte (append ex) = ret [] (x::xs)
 Proof
-  qspec_then ‘[]’ mp_tac widget0_rest \\ simp[]
+  qspec_then ‘[]’ mp_tac dess0r \\ simp[]
 QED
 
-Triviality widget1_rest:
+
+Triviality dess1r:
   ∀rest x xs ex.
     enc_section 1w enc_ass (x::xs) = SOME ex ⇒
     dec_section 1w dec_ass (ex a++ rest) = ret rest (x::xs)
 Proof
      rpt strip_tac
-  >> imp_res_tac enc_section_nEmp
-  >> assume_tac dec_enc_ass
-  >> imp_res_tac dec_enc_section
-  >> pop_assum $ qspec_then ‘rest’ mp_tac
-  >> simp[]
+  \\ imp_res_tac enc_section_nEmp__nNUL
+  \\ assume_tac dec_enc_ass
+  \\ imp_res_tac dec_enc_section
+  \\ pop_assum $ qspec_then ‘rest’ mp_tac
+  \\ simp[]
 QED
 
-Triviality widget1:
+Triviality dess1:
   ∀x xs ex.
     enc_section 1w enc_ass (x::xs) = SOME ex ⇒
     dec_section 1w dec_ass (append ex) = ret [] (x::xs)
 Proof
-  qspec_then ‘[]’ mp_tac widget1_rest \\ simp[]
+  qspec_then ‘[]’ mp_tac dess1r \\ simp[]
 QED
 
-Triviality widget2:
+
+Triviality dess2:
   ∀x xs ex.
     enc_section 2w (enc_idx_alpha enc_map) (x::xs) = SOME ex ⇒
     dec_section 2w (dec_idx_alpha dec_map) (append ex) = ret [] (x::xs)
 Proof
      rpt strip_tac
-  \\ imp_res_tac enc_section_nEmp
+  \\ imp_res_tac enc_section_nEmp__nNUL
   \\ assume_tac dec_enc_map
   \\ dxrule_at Any dec_enc_idx_alpha
   \\ strip_tac
   \\ imp_res_tac dec_enc_section_NR
 QED
 
-Triviality widget_1_rest:
+
+
+
+
+(* dec-enc section thms used in the module proof *)
+Triviality des1r:
   ∀rest x xs ex.
     enc_section 1w enc_functype (x::xs) = SOME ex ⇒
     dec_section 1w dec_functype (ex a++ rest) = ret rest (x::xs)
 Proof
      rpt strip_tac
-  >> imp_res_tac enc_section_nEmp
-  >> assume_tac dec_enc_functype
-  >> imp_res_tac dec_enc_section
-  >> pop_assum $ qspec_then ‘rest’ mp_tac
-  >> simp[]
+  \\ imp_res_tac enc_section_nEmp__nNUL
+  \\ assume_tac dec_enc_functype
+  \\ imp_res_tac dec_enc_section
+  \\ pop_assum $ qspec_then ‘rest’ mp_tac
+  \\ simp[]
 QED
 
-Triviality widget_1:
+Triviality des1:
   ∀x xs es.
   enc_section 1w enc_functype (x::xs) = SOME es ⇒
   dec_section 1w dec_functype (append es) = ret [] (x::xs)
 Proof
-  qspec_then ‘[]’ mp_tac widget_1_rest \\ simp[]
+  qspec_then ‘[]’ mp_tac des1r \\ simp[]
 QED
 
-Triviality widget3_rest:
+
+Triviality des3r:
   ∀rest x xs es.
     enc_section 3w enc_u32 (x::xs) = SOME es ⇒
     dec_section 3w dec_u32 (es a++ rest) = ret rest (x::xs)
 Proof
      rpt strip_tac
-  >> imp_res_tac enc_section_nEmp
-  >> assume_tac dec_enc_u32
-  >> imp_res_tac dec_enc_section
-  >> pop_assum $ qspec_then ‘rest’ mp_tac
-  >> simp[]
+  \\ imp_res_tac enc_section_nEmp__nNUL
+  \\ assume_tac dec_enc_u32
+  \\ imp_res_tac dec_enc_section
+  \\ pop_assum $ qspec_then ‘rest’ mp_tac
+  \\ simp[]
 QED
 
-Triviality widget3:
+Triviality des3:
   ∀rest x xs es.
     enc_section 3w enc_u32 (x::xs) = SOME es ⇒
     dec_section 3w dec_u32 (append es) = ret [] (x::xs)
 Proof
-  qspec_then ‘[]’ mp_tac widget3_rest \\ simp[]
+  qspec_then ‘[]’ mp_tac des3r \\ simp[]
 QED
 
-Triviality widget5_rest:
+Triviality des5r:
   ∀rest x xs es.
     enc_section 5w enc_limits (x::xs) = SOME es ⇒
     dec_section 5w dec_limits (es a++ rest) = ret rest (x::xs)
 Proof
      rpt strip_tac
-  >> imp_res_tac enc_section_nEmp
+  >> imp_res_tac enc_section_nEmp__nNUL
   >> assume_tac dec_enc_limits
   >> imp_res_tac dec_enc_section
   >> pop_assum $ qspec_then ‘rest’ mp_tac
   >> simp[]
 QED
 
-Triviality widget5:
+Triviality des5:
   ∀rest x xs es.
     enc_section 5w enc_limits (x::xs) = SOME es ⇒
     dec_section 5w dec_limits (append es) = ret [] (x::xs)
 Proof
-  qspec_then ‘[]’ mp_tac widget5_rest \\ simp[]
+  qspec_then ‘[]’ mp_tac des5r \\ simp[]
 QED
 
-Triviality widget6_rest:
+Triviality des6r:
   ∀rest x xs es.
     enc_section 6w enc_global (x::xs) = SOME es ⇒
     dec_section 6w dec_global (es a++ rest) = ret rest (x::xs)
 Proof
      rpt strip_tac
-  >> imp_res_tac enc_section_nEmp
+  >> imp_res_tac enc_section_nEmp__nNUL
   >> assume_tac dec_enc_global
   >> imp_res_tac dec_enc_section
   >> pop_assum $ qspec_then ‘rest’ mp_tac
   >> simp[]
 QED
 
-Triviality widget6:
+Triviality des6:
   ∀rest x xs es.
     enc_section 6w enc_global (x::xs) = SOME es ⇒
     dec_section 6w dec_global (append es) = ret [] (x::xs)
 Proof
-  qspec_then ‘[]’ mp_tac widget6_rest \\ simp[]
+  qspec_then ‘[]’ mp_tac des6r \\ simp[]
 QED
 
 
-Triviality widget10_rest:
+Triviality des10r:
   ∀rest x xs es.
     enc_section 10w enc_code (x::xs) = SOME es ⇒
     dec_section 10w dec_code (es a++ rest) = ret rest (x::xs)
 Proof
      rpt strip_tac
-  >> imp_res_tac enc_section_nEmp
+  >> imp_res_tac enc_section_nEmp__nNUL
   >> assume_tac dec_enc_code
   >> imp_res_tac dec_enc_section
   >> pop_assum $ qspec_then ‘rest’ mp_tac
   >> simp[]
 QED
 
-Triviality widget10:
+Triviality des10:
   ∀rest x xs es.
     enc_section 10w enc_code (x::xs) = SOME es ⇒
     dec_section 10w dec_code (append es) = ret [] (x::xs)
 Proof
-  qspec_then ‘[]’ mp_tac widget10_rest \\ simp[]
+  qspec_then ‘[]’ mp_tac des10r \\ simp[]
 QED
 
-Triviality widget11_rest:
+Triviality des11r:
   ∀rest x xs es.
     enc_section 11w enc_data (x::xs) = SOME es ⇒
     dec_section 11w dec_data (es a++ rest) = ret rest (x::xs)
 Proof
      rpt strip_tac
-  >> imp_res_tac enc_section_nEmp
+  >> imp_res_tac enc_section_nEmp__nNUL
   >> assume_tac dec_enc_data
   >> imp_res_tac dec_enc_section
   >> pop_assum $ qspec_then ‘rest’ mp_tac
@@ -1225,35 +1296,36 @@ Proof
 QED
 
 
-Triviality widget11:
+Triviality des11:
   ∀x xs es.
     enc_section 11w enc_data (x::xs) = SOME es ⇒
     dec_section 11w dec_data (append es) = ret [] (x::xs)
 Proof
-  qspec_then ‘[]’ mp_tac widget11_rest \\ simp[]
+  qspec_then ‘[]’ mp_tac des11r \\ simp[]
 QED
 
 
 
+
+(* pass through thms; saying that if trying to decode a X from the bytecode of a Y results in a no-op *)
 Triviality pt12:
   ∀x xs ss2.
     enc_section 2w (enc_idx_alpha enc_map) (x::xs) = SOME ss2 ⇒
     dec_section 1w dec_ass (append ss2) = ret (append ss2) []
 Proof
      rpt strip_tac
-  >> qspecl_then [‘1w’, ‘dec_ass’] (drule_at Any) enc_dec_section_passThrough
+  >> qspecl_then [‘1w’, ‘dec_ass’] (drule_at Any) enc_dec_section_pt
   >> simp[]
 QED
 
 
-
-Triviality pt0_rest:
+Triviality pt0r:
   ∀rest b enc x xs es. b ≠ 0w ∧
     enc_section b enc (x::xs) = SOME es ⇒
     dec_section 0w dec_byte (es a++ rest) = ret (es a++ rest) []
 Proof
      rpt strip_tac
-  \\ qspecl_then [‘0w’, ‘dec_byte’, ‘b’, ‘enc’] dxrule_all enc_dec_section_passThrough_rest
+  \\ qspecl_then [‘0w’, ‘dec_byte’, ‘b’, ‘enc’] dxrule_all enc_dec_section_ptr
   \\ simp[]
 QED
 
@@ -1263,20 +1335,18 @@ Triviality pt0:
     dec_section 0w dec_byte (append es) = ret (append es) []
 Proof
      rpt strip_tac
-  \\ qspec_then ‘[]’ dxrule_all pt0_rest
+  \\ qspec_then ‘[]’ dxrule_all pt0r
   \\ simp[]
 QED
 
 
-
-
-Triviality pt1_rest:
+Triviality pt1r:
   ∀rest b enc x xs es. b ≠ 1w ∧
   enc_section b enc (x::xs) = SOME es ⇒
   dec_section 1w dec_functype (es a++ rest) = ret (es a++ rest) []
 Proof
      rpt strip_tac
-  >> qspecl_then [‘1w’, ‘dec_functype’, ‘b’, ‘enc’] (drule_at Any) enc_dec_section_passThrough_rest
+  >> qspecl_then [‘1w’, ‘dec_functype’, ‘b’, ‘enc’] (drule_at Any) enc_dec_section_ptr
   >> simp[]
 QED
 
@@ -1286,18 +1356,18 @@ Triviality pt1:
     dec_section 1w dec_functype (append es) = ret (append es) []
 Proof
      rpt strip_tac
-  >> qspec_then ‘[]’ (drule_at Any) pt1_rest
+  >> qspec_then ‘[]’ (drule_at Any) pt1r
   >> simp[]
 QED
 
 
-Triviality pt3_rest:
+Triviality pt3r:
   ∀rest b enc x xs es. b ≠ 3w ∧
     enc_section b enc (x::xs) = SOME es ⇒
     dec_section 3w dec_u32 (es a++ rest) = ret (es a++ rest) []
 Proof
      rpt strip_tac
-  >> qspecl_then [‘3w’, ‘dec_u32’, ‘b’, ‘enc’] (drule_at Any) enc_dec_section_passThrough_rest
+  >> qspecl_then [‘3w’, ‘dec_u32’, ‘b’, ‘enc’] (drule_at Any) enc_dec_section_ptr
   >> simp[]
 QED
 
@@ -1307,17 +1377,18 @@ Triviality pt3:
     dec_section 3w dec_u32 (append es) = ret (append es) []
 Proof
      rpt strip_tac
-  >> qspec_then ‘[]’ (drule_at Any) pt3_rest
+  >> qspec_then ‘[]’ (drule_at Any) pt3r
   >> simp[]
 QED
 
-Triviality pt5_rest:
+
+Triviality pt5r:
   ∀rest b enc x xs es. b ≠ 5w ∧
     enc_section b enc (x::xs) = SOME es ⇒
     dec_section 5w dec_limits (es a++ rest) = ret (es a++ rest) []
 Proof
      rpt strip_tac
-  >> qspecl_then [‘5w’, ‘dec_limits’, ‘b’, ‘enc’] (drule_at Any) enc_dec_section_passThrough_rest
+  >> qspecl_then [‘5w’, ‘dec_limits’, ‘b’, ‘enc’] (drule_at Any) enc_dec_section_ptr
   >> simp[]
 QED
 
@@ -1327,17 +1398,18 @@ Triviality pt5:
     dec_section 5w dec_limits (append es) = ret (append es) []
 Proof
      rpt strip_tac
-  >> qspec_then ‘[]’ (drule_at Any) pt5_rest
+  >> qspec_then ‘[]’ (drule_at Any) pt5r
   >> simp[]
 QED
 
-Triviality pt6_rest:
+
+Triviality pt6r:
   ∀rest b enc x xs es. b ≠ 6w ∧
     enc_section b enc (x::xs) = SOME es ⇒
     dec_section 6w dec_global (es a++ rest) = ret (es a++ rest) []
 Proof
      rpt strip_tac
-  >> qspecl_then [‘6w’, ‘dec_global’, ‘b’, ‘enc’] (drule_at Any) enc_dec_section_passThrough_rest
+  >> qspecl_then [‘6w’, ‘dec_global’, ‘b’, ‘enc’] (drule_at Any) enc_dec_section_ptr
   >> simp[]
 QED
 
@@ -1347,19 +1419,18 @@ Triviality pt6:
     dec_section 6w dec_global (append es) = ret (append es) []
 Proof
      rpt strip_tac
-  >> qspec_then ‘[]’ (drule_at Any) pt6_rest
+  >> qspec_then ‘[]’ (drule_at Any) pt6r
   >> simp[]
 QED
 
 
-
-Triviality pt10_rest:
+Triviality pt10r:
   ∀rest b enc x xs es. b ≠ 10w ∧
     enc_section b enc (x::xs) = SOME es ⇒
     dec_section 10w dec_code (es a++ rest) = ret (es a++ rest) []
 Proof
      rpt strip_tac
-  >> qspecl_then [‘10w’, ‘dec_code’, ‘b’, ‘enc’] (drule_at Any) enc_dec_section_passThrough_rest
+  >> qspecl_then [‘10w’, ‘dec_code’, ‘b’, ‘enc’] (drule_at Any) enc_dec_section_ptr
   >> simp[]
 QED
 
@@ -1369,12 +1440,9 @@ Triviality pt10:
     dec_section 10w dec_code (append es) = ret (append es) []
 Proof
      rpt strip_tac
-  >> qspec_then ‘[]’ (drule_at Any) pt10_rest
+  >> qspec_then ‘[]’ (drule_at Any) pt10r
   >> simp[]
 QED
-
-
-
 
 
 
@@ -1384,75 +1452,75 @@ QED
 (*   Pass through, names section   *)
 (***********************************)
 
-Triviality ptns_1:
+Triviality ptns1:
   ∀x ex.
     enc_names_section x = SOME ex ⇒
     dec_section 1w dec_functype (append ex) = ret (append ex) []
 Proof
      rpt strip_tac
-  \\ ‘x = blank_names ∨ x ≠ blank_names’ by simp[]
+  \\ Cases_on ‘x = blank_names’
   >- gvs[]
-  \\ imp_res_tac enc_names_section_nEmp'
+  \\ imp_res_tac enc_names_section_not_blank__lbn0
   >> rw[oneline dec_section_def]
 QED
 
-Triviality ptns_3:
+Triviality ptns3:
   ∀x ex.
     enc_names_section x = SOME ex ⇒
     dec_section 3w dec_u32 (append ex) = ret (append ex) []
 Proof
      rpt strip_tac
-  \\ ‘x = blank_names ∨ x ≠ blank_names’ by simp[]
+  \\ Cases_on ‘x = blank_names’
   >- gvs[]
-  \\ imp_res_tac enc_names_section_nEmp'
+  \\ imp_res_tac enc_names_section_not_blank__lbn0
   >> rw[oneline dec_section_def]
 QED
 
-Triviality ptns_5:
+Triviality ptns5:
   ∀x ex.
     enc_names_section x = SOME ex ⇒
     dec_section 5w dec_limits (append ex) = ret (append ex) []
 Proof
      rpt strip_tac
-  \\ ‘x = blank_names ∨ x ≠ blank_names’ by simp[]
+  \\ Cases_on ‘x = blank_names’
   >- gvs[]
-  \\ imp_res_tac enc_names_section_nEmp'
+  \\ imp_res_tac enc_names_section_not_blank__lbn0
   >> rw[oneline dec_section_def]
 QED
 
-Triviality ptns_6:
+Triviality ptns6:
   ∀x ex.
     enc_names_section x = SOME ex ⇒
     dec_section 6w dec_global (append ex) = ret (append ex) []
 Proof
      rpt strip_tac
-  \\ ‘x = blank_names ∨ x ≠ blank_names’ by simp[]
+  \\ Cases_on ‘x = blank_names’
   >- gvs[]
-  \\ imp_res_tac enc_names_section_nEmp'
+  \\ imp_res_tac enc_names_section_not_blank__lbn0
   >> rw[oneline dec_section_def]
 QED
 
-Triviality ptns_10:
+Triviality ptns10:
   ∀x ex.
     enc_names_section x = SOME ex ⇒
     dec_section 10w dec_code (append ex) = ret (append ex) []
 Proof
      rpt strip_tac
-  \\ ‘x = blank_names ∨ x ≠ blank_names’ by simp[]
+  \\ Cases_on ‘x = blank_names’
   >- gvs[]
-  \\ imp_res_tac enc_names_section_nEmp'
+  \\ imp_res_tac enc_names_section_not_blank__lbn0
   >> rw[oneline dec_section_def]
 QED
 
-Triviality ptns_11:
+Triviality ptns11:
   ∀x ex.
     enc_names_section x = SOME ex ⇒
     dec_section 11w dec_data (append ex) = ret (append ex) []
 Proof
      rpt strip_tac
-  \\ ‘x = blank_names ∨ x ≠ blank_names’ by simp[]
+  \\ Cases_on ‘x = blank_names’
   >- gvs[]
-  \\ imp_res_tac enc_names_section_nEmp'
+  \\ imp_res_tac enc_names_section_not_blank__lbn0
   >> rw[oneline dec_section_def]
 QED
 
@@ -1471,7 +1539,7 @@ Proof
   \\ namedCases_on ‘s’ ["", "s ss"]
   >> namedCases_on ‘f_names’ ["", "f fs"]
   >> namedCases_on ‘l_names’ ["", "l ls"]
-    >> rw $ ssaa [enc_names_section_def, prepend_sz_def, string2bytes_def, blank_names_values]
+    >> rw $ ssaa [enc_names_section_def, prepend_B_sz_def, string2bytes_def, blank_names_values]
     (* get encoders in the right shape *)
     >> ifHyp ‘SOME _ = enc_u32 _         ’ $ assume_tac o GSYM
     >> ifHyp ‘SOME _ = enc_section 0w _ _’ $     mp_tac o GSYM
@@ -1481,21 +1549,21 @@ Proof
     *)
     (* magic bytes & prepended size *)
     >> imp_res_tac dec_enc_u32
-    >> imp_res_tac enc_section_nEmp
+    >> imp_res_tac enc_section_nEmp__nNUL
     (* decode various sections, based on whether they're present or not *)
-    >> gvs $ ssaa [dec_names_section_def, magic_bytes_def, string2bytes_def]
+    >> gvs $ ssaa [dec_names_section_def, name_bytes_def, string2bytes_def]
     >> gvs $ [GSYM LENGTH_APPEND, Excl "LENGTH_APPEND", TAKE_LENGTH_APPEND]
     >> simp ssa
     (**)
     >> imp_res_tac pt0      (* imp_res_tac only fires if antecedent is present *)
-    >> imp_res_tac pt0_rest (* for any given goal, some of these hyps may be superfluous *)
+    >> imp_res_tac pt0r (* for any given goal, some of these hyps may be superfluous *)
     >> imp_res_tac pt12
     (**)
-    >> imp_res_tac widget0
-    >> imp_res_tac widget1
-    >> imp_res_tac widget2
-    >> imp_res_tac widget0_rest
-    >> imp_res_tac widget1_rest
+    >> imp_res_tac dess0
+    >> imp_res_tac dess1
+    >> imp_res_tac dess2
+    >> imp_res_tac dess0r
+    >> imp_res_tac dess1r
     (**)
     >> fs[names_component_equality, DROP_LENGTH_APPEND, GSYM LENGTH_APPEND, Excl "LENGTH_APPEND"]
 QED
@@ -1505,7 +1573,7 @@ Theorem dec_enc_names_NE: (* not empty *)
     n ≠ blank_names ∧ enc_names_section n = SOME encn ⇒
     dec_names_section $ encn a++ rest = ret rest [n]
 Proof
-     ntac 4 $ strip_tac
+     ntac 4 strip_tac
   \\ imp_res_tac dec_enc_names
   \\ gvs[]
 QED
@@ -1516,7 +1584,7 @@ Theorem dec_enc_names_NR: (* no rest *)
     dec_names_section $ append encn = ret [] [n]
 Proof
      rpt strip_tac
-  \\ ‘n = blank_names ∨ n ≠ blank_names’ by simp[]
+  \\ Cases_on ‘n = blank_names’
   >-(
        rw[oneline dec_names_section_def]
     >> assume_tac enc_names_section_blank
@@ -1541,30 +1609,30 @@ Proof
   >> namedCases_on ‘globals’ ["","g gs"]
   >> namedCases_on ‘datas’   ["","d ds"]
     >> gvs[blank_mod_def, enc_mod_and_names_def, dec_mod_and_names_def, split_funcs_def]
-    >> imp_res_tac enc_section_nEmp
+    >> imp_res_tac enc_section_nEmp__nNUL
     >> gvs[mod_leader_def]
     (**)
     >> imp_res_tac pt1
-    >> imp_res_tac pt1_rest
+    >> imp_res_tac pt1r
     >> imp_res_tac pt3
-    >> imp_res_tac pt3_rest
+    >> imp_res_tac pt3r
     >> imp_res_tac pt5
-    >> imp_res_tac pt5_rest
+    >> imp_res_tac pt5r
     >> imp_res_tac pt6
-    >> imp_res_tac pt6_rest
+    >> imp_res_tac pt6r
     >> imp_res_tac pt10
     (**)
-    >> imp_res_tac widget11
-    >> imp_res_tac widget10_rest
-    >> imp_res_tac widget10
-    >> imp_res_tac widget6_rest
-    >> imp_res_tac widget6
-    >> imp_res_tac widget5_rest
-    >> imp_res_tac widget5
-    >> imp_res_tac widget3_rest
-    >> imp_res_tac widget3
-    >> imp_res_tac widget_1_rest
-    >> imp_res_tac widget_1
+    >> imp_res_tac des11
+    >> imp_res_tac des10r
+    >> imp_res_tac des10
+    >> imp_res_tac des6r
+    >> imp_res_tac des6
+    >> imp_res_tac des5r
+    >> imp_res_tac des5
+    >> imp_res_tac des3r
+    >> imp_res_tac des3
+    >> imp_res_tac des1r
+    >> imp_res_tac des1
     (**)
     >> simp ssa
     >> simp [module_component_equality, func_component_equality, zip_funcs_def, split_zip_funcs]
@@ -1575,8 +1643,8 @@ Theorem dec_enc_mod_and_names:
     enc_mod_and_names mod nms = SOME emn ⇒
     dec_mod_and_names $ append emn = ret [] (mod,nms)
 Proof
-  rpt strip_tac
-  \\ ‘nms = blank_names ∨ nms ≠ blank_names’ by simp[]
+     rpt strip_tac
+  \\ Cases_on ‘nms = blank_names’
   >- gvs[dec_enc_module]
   \\ namedCases_on ‘mod’ ["types funcs mems globals datas"]
   >> namedCases_on ‘funcs’   ["","f fs"]
@@ -1586,84 +1654,43 @@ Proof
   >> namedCases_on ‘globals’ ["","g gs"]
   >> namedCases_on ‘datas’   ["","d ds"]
     >> gvs[blank_mod_def, enc_mod_and_names_def, dec_mod_and_names_def, split_funcs_def]
-    >> imp_res_tac enc_section_nEmp
-    >> imp_res_tac enc_names_section_nEmp
+    >> imp_res_tac enc_section_nEmp__nNUL
+    >> imp_res_tac enc_names_section_not_blank__nNUL
     >> gvs[mod_leader_def]
     (**)
     >> imp_res_tac pt1
-    >> imp_res_tac pt1_rest
     >> imp_res_tac pt3
-    >> imp_res_tac pt3_rest
     >> imp_res_tac pt5
-    >> imp_res_tac pt5_rest
     >> imp_res_tac pt6
-    >> imp_res_tac pt6_rest
     >> imp_res_tac pt10
-    >> imp_res_tac pt10_rest
+    >> imp_res_tac pt1r
+    >> imp_res_tac pt3r
+    >> imp_res_tac pt5r
+    >> imp_res_tac pt6r
+    >> imp_res_tac pt10r
     (**)
-    >> imp_res_tac widget11_rest
-    >> imp_res_tac widget11
-    >> imp_res_tac widget10_rest
-    >> imp_res_tac widget10
-    >> imp_res_tac widget6_rest
-    >> imp_res_tac widget6
-    >> imp_res_tac widget5_rest
-    >> imp_res_tac widget5
-    >> imp_res_tac widget3_rest
-    >> imp_res_tac widget3
-    >> imp_res_tac widget_1_rest
-    >> imp_res_tac widget_1
+    >> imp_res_tac des11r
+    >> imp_res_tac des10r
+    >> imp_res_tac des6r
+    >> imp_res_tac des5r
+    >> imp_res_tac des3r
+    >> imp_res_tac des1r
+    >> imp_res_tac des11
+    >> imp_res_tac des10
+    >> imp_res_tac des6
+    >> imp_res_tac des5
+    >> imp_res_tac des3
+    >> imp_res_tac des1
     (**)
-    >> imp_res_tac ptns_1
-    >> imp_res_tac ptns_3
-    >> imp_res_tac ptns_5
-    >> imp_res_tac ptns_6
-    >> imp_res_tac ptns_10
-    >> imp_res_tac ptns_11
+    >> imp_res_tac ptns1
+    >> imp_res_tac ptns3
+    >> imp_res_tac ptns5
+    >> imp_res_tac ptns6
+    >> imp_res_tac ptns10
+    >> imp_res_tac ptns11
     >> imp_res_tac dec_enc_names_NR
     (**)
     >> simp ssa
     >> simp [module_component_equality, func_component_equality, zip_funcs_def, split_zip_funcs]
 QED
 
-
-(*
-Triviality foo:
-  ∀n encn xs len.
-  n ≠ blank ∧
-  enc_names_section n = SOME encn ⇒
-  ∃xs.
-  append encn = 0w :: xs ∧ ∃ys len.
-  dec_u32 xs = ret ys len
-Proof
-  ntac 5 $ strip_tac
-  \\ imp_res_tac enc_names_section_nEmp
-  >> imp_res_tac names_not_blank'
-  >> gvs[enc_names_section_def]
-  >> imp_res_tac enc_section_nEmp'
-  >> gvs[prepend_sz_def]
-  >> imp_res_tac dec_enc_u32
-  >> rewrite_tac ssa
-  >> pop_assum $ qspec_then ‘magic_bytes ++ ss0 a++ ss1 a++ append ss2’ assume_tac
-  >> simp[]
-QED
-*)
-
-(*
-MAP_MAPi
-MAP_MAP_o
-MAP_o
-MAP_COMPOSE
-*)
-
-
-(*
-Triviality enc_names_section_nEmp:
-  ∀x.
-  x ≠ blank_names ⇒ ∃encx.
-  enc_names_section x = SOME encx
-Proof
-  Cases
-  rw[enc_names_section_def]
-QED
-*)
